theories/simplang/tactics.v
@@ -60,5 +60,5 @@ Global Hint Extern 0 (head_reducible _ _ _) => eexists _, _; simpl : head_step.
 
 (* [simpl apply] is too stupid, so we need extern hints here. *)
 Global Hint Extern 1 (head_step _ _ _ _ _) => econstructor : head_step.
-Global Hint Extern 0 (head_step _ (CmpXchg _ _ _) _ _ _) => eapply CmpXchgS : head_step.
-Global Hint Extern 0 (head_step _ (AllocN _ _) _ _ _) => apply alloc_fresh : head_step.
+(*Global Hint Extern 0 (head_step _ (CmpXchg _ _ _) _ _ _) => eapply CmpXchgS : head_step.*)
+(*Global Hint Extern 0 (head_step _ (AllocN _ _) _ _ _) => apply alloc_fresh : head_step.*)
